concurrency/bst_conc_nblocking2_spec.v
@@ -6,7 +6,7 @@ Require Import VST.atomics.general_locks.
 Require Import VST.atomics.SC_atomics.
 Require Import Coq.Sets.Ensembles.
 Require Import VST.msl.iter_sepcon.
-Require Import bst.bst_conc_nblocking2.
+Require Import bst.bst_conc_nblocking4.
 
 
 Definition atomic_ptr := Tstruct _atom_ptr noattr.
@@ -14,6 +14,7 @@ Variable atomic_ptr_at : share -> val -> val -> mpred.
 Hypothesis atomic_ptr_at__ : forall sh v p, atomic_ptr_at sh v p |-- atomic_ptr_at sh Vundef p.
 Definition t_struct_tree := Tstruct _tree noattr.
 (* Definition t_struct_list := Tstruct _list noattr. *)
+Definition t_struct_operation := Tstruct _operation noattr.
 Definition t_struct_child_cas_operation := Tstruct _child_cas_operation noattr.
 Definition t_struct_relocate_operation := Tstruct _relocate_operation noattr.
 (* Definition t_arr := Tarray (tptr t_struct_list ) 5 noattr. *)
@@ -39,82 +40,79 @@ Definition Vprog : varspecs. mk_varspecs prog. Defined.
        SEP (mem_mgr gv; malloc_token Ews t p * data_at_ Ews t p). *)
 
 
-Fixpoint ghost_tree_rep (t: @ ghost_tree val ) (nb:val) (g_current:gname) (g:gname) range : mpred := 
+Fixpoint ghost_tree_rep (t: @ ghost_op_tree val ) (nb:val) (g_current:gname) (g:gname) (g_op:gname) range : mpred := 
  match t, range with
- | E_ghost , _ => atomic_ptr_at Ews nullval nb * ghost_master1 (ORD := range_order)  (range,  (@None ghost_info)) g_current 
- | (T_ghost a ga lp x v vp op b gb rp ), (l, r) =>  EX tp, EX sh, !!(readable_share sh  /\ Int.min_signed <= x <= Int.max_signed/\ is_pointer_or_null lp /\ is_pointer_or_null rp /\ is_pointer_or_null vp  ) &&  atomic_ptr_at Ews tp nb * atomic_ptr_at Ews v vp * malloc_token Ews t_struct_tree tp * data_at sh t_struct_tree (Vint (Int.repr x),(vp,(op,(lp,rp)))) tp *
-  ghost_master1 (ORD := range_order)  (range,  (@Some ghost_info (x,vp,ga,gb))) g_current * in_tree ga (l, Finite_Integer x) lp g * in_tree gb ( Finite_Integer x, r) rp g *  ghost_tree_rep a  lp ga g (l, Finite_Integer x) * ghost_tree_rep b rp gb g (Finite_Integer x, r)
- end.
+ | E_op , _ => atomic_ptr_at Ews nullval nb * ghost_master1 (ORD := range_order)  (range,  (@None ghost_info)) g_current 
+ | (T_op a ga lp x v vp o aop b gb rp ), (l, r) =>  (EX tp, EX op, EX sh, !!(readable_share sh  /\ Int.min_signed <= x <= Int.max_signed/\ is_pointer_or_null lp /\ is_pointer_or_null rp /\ is_pointer_or_null vp  ) && 
+   atomic_ptr_at Ews tp nb * atomic_ptr_at Ews v vp * atomic_ptr_at Ews op aop *
+  (match o with | Some o' => in_tree_op g_op o' *  match o' with |ADD_op b' x' v' => EX rop, EX t, EX e, EX u, EX vp', EX aop', EX lp', EX rp', EX op', malloc_token Ews t_struct_operation op * data_at Ews t_struct_operation (rop, Vint (Int.repr t)) op * data_at Ews t_struct_child_cas_operation (Vint (Int.repr (if(b') then 1 else 0 )), (e, u)) rop 
+  																																									* data_at sh t_struct_tree (Vint (Int.repr x'),(vp',(aop',(lp',rp')))) u * atomic_ptr_at Ews v' vp' * atomic_ptr_at Ews op' aop' * data_at Ews t_struct_operation (nullval, Vint (Int.repr 0)) op' * atomic_ptr_at Ews nullval lp' * atomic_ptr_at Ews nullval rp' 
+                                           | DELETE_op b' x' => EX rop, EX t, malloc_token Ews t_struct_operation op * data_at Ews t_struct_operation (rop, Vint (Int.repr t)) op  end
+                | None => !!(op = nullval) && emp end) * 
+   data_at sh t_struct_tree (Vint (Int.repr x),(vp,(aop,(lp,rp)))) tp * malloc_token Ews t_struct_tree tp *
+   ghost_master1 (ORD := range_order)  (range,  (@Some ghost_info (x,vp,ga,gb))) g_current *
+   in_tree ga (l, Finite_Integer x) lp g * in_tree gb ( Finite_Integer x, r) rp g *
+   ghost_tree_rep a  lp ga g g_op(l, Finite_Integer x) * ghost_tree_rep b rp gb g g_op (Finite_Integer x, r)
+  ) end.
 
-Definition tree_rep2 (g:gname) (g_root: gname) (nb:val) (sh:share) (t: @tree val  ) : mpred := EX (tg:ghost_tree), !! (find_pure_tree tg = t) && ghost_tree_rep tg  nb g_root g (Neg_Infinity, Pos_Infinity) 
-                                                                                                                                 * bst_conc_lemmas2.ghost_ref g (find_ghost_set tg g_root ( Neg_Infinity, Pos_Infinity) nb).
 
-Definition nodebox_rep (sh : share) (nb: val) (g_root: gname) (g:gname)  :=  EX tp:val, EX lp: list val,  atomic_ptr_at sh tp nb * iter_sepcon ( fun p => EX sh1:share, data_at_ sh1 t_struct_tree p ) lp * in_tree g_root (Neg_Infinity, Pos_Infinity) nb g.
+Definition tree_rep2 (g:gname) (g_op:gname) (g_root:gname) (nb:val) (sh:share) (t: @tree val  ) : mpred := EX (tg:ghost_op_tree), !! (find_pure_tree2 tg = t) && ghost_tree_rep tg  nb g_root g g_op (Neg_Infinity, Pos_Infinity) 
+                                                                                                                                 * bst_conc_lemmas2.ghost_ref g (find_ghost_set2 tg g_root ( Neg_Infinity, Pos_Infinity) nb) 
+                                                                                                                                 * bst_conc_lemmas2.ghost_ref_op g_op (find_op_set tg).                                    
+
+
+Definition nodebox_rep (sh : share) (nb: val) ( rnb: val) (g_root: gname) (g:gname)  :=  EX tp:val, EX rtp:val, EX vp:val, EX aop:val, EX lp:val,  EX lop: list val,  atomic_ptr_at sh tp nb * malloc_token Ews t_struct_tree tp * data_at sh t_struct_tree (Vint (Int.repr (-1)),(vp,(aop,(lp,rnb)))) tp *  atomic_ptr_at sh rtp rnb * iter_sepcon ( fun p => EX sh1:share, data_at_ sh1 t_struct_tree p ) lop * in_tree g_root (Neg_Infinity, Pos_Infinity) rnb g.
 
 Program Definition find_spec :=
   DECLARE _find
-  ATOMIC TYPE (rmaps.ConstType ( val * share* Z * val * val * val * val * Z * val * globals * gname * gname))
+  ATOMIC TYPE (rmaps.ConstType ( val * val * share* Z * val * val * val * val * Z * val * globals * gname * gname * gname))
          OBJ BST INVS base.empty base.top
-  WITH b, sh, x, pred, pred_op, curr, curr_op, n, v, gv, g, g_root
+  WITH b, nb, sh, x, pred, pred_op, curr, curr_op, n, v, gv, g, g_op, g_root
   PRE [ _key OF tint, _pred OF (tptr (tptr atomic_ptr)), _pred_op OF (tptr (tptr tvoid)), _curr OF (tptr (tptr atomic_ptr)), _curr_op OF (tptr (tptr tvoid)), _auxRoot OF (tptr atomic_ptr), _thread_num OF tint, _v OF (tptr (tptr tvoid)) ]
     PROP (
           Int.min_signed <= x <= Int.max_signed)
     LOCAL (temp _auxRoot b; temp _key (Vint (Int.repr x)); temp _pred pred; temp _pred pred; temp _pred_op pred_op; temp _curr curr; temp _curr_op curr_op; temp _thread_num (Vint (Int.repr n)); temp _v v; gvars gv)
-    SEP  (mem_mgr gv; nodebox_rep sh b g_root g) |
-  (!! sorted_tree BST && data_at_ Ews (tptr tvoid) v * tree_rep2 g g_root b sh BST)
+    SEP  (mem_mgr gv; nodebox_rep sh b nb g_root g) |
+  (!! sorted_tree BST && data_at_ Ews (tptr tvoid) v * tree_rep2 g g_op g_root nb sh BST)
   POST [tint ]
     EX ret: Z,
     PROP ()
     LOCAL (temp ret_temp (vint ret))
-    SEP (mem_mgr gv; nodebox_rep sh b g_root g) |
-        ( EX vp:val,  !! (sorted_tree BST /\ (if eq_dec ret 3 then vp <> Vundef else vp <> Vundef ) /\ vp = (bst_conc_lemmas2.lookup nullval x BST)) &&  data_at Ews (tptr tvoid) vp v * tree_rep2 g g_root b sh BST).
-
+    SEP (mem_mgr gv; nodebox_rep sh b nb g_root g) |
+        ( EX vp:val,  !! (sorted_tree BST /\ (if eq_dec ret 3 then vp <> Vundef else vp <> Vundef ) /\ vp = (bst_conc_lemmas2.lookup nullval x BST)) &&  data_at Ews (tptr tvoid) vp v * tree_rep2 g g_op g_root nb sh BST).
+ 
 Program Definition add_spec :=
   DECLARE _add
-  ATOMIC TYPE (rmaps.ConstType ( share* Z * Z * val * globals * gname * gname))
+  ATOMIC TYPE (rmaps.ConstType ( val * share* Z * Z * val * globals * gname * gname * gname))
          OBJ BST INVS base.empty base.top
-  WITH  sh, x,  n, v, gv, g, g_root
+  WITH  nb, sh, x,  n, v, gv, g, g_op, g_root
   PRE [ _key OF tint,  _value OF (tptr tvoid), _thread_num OF tint ]
     PROP (
           Int.min_signed <= x <= Int.max_signed)
     LOCAL (temp _key (Vint (Int.repr x)); temp _thread_num (Vint (Int.repr n)); temp _value v; gvars gv)
-    SEP  (mem_mgr gv; nodebox_rep sh (gv _base_root) g_root g) |(!! sorted_tree BST && tree_rep2 g g_root (gv _base_root) sh BST)
+    SEP  (mem_mgr gv; nodebox_rep sh (gv _base_root) nb g_root g) |(!! sorted_tree BST && tree_rep2 g g_op g_root nb sh BST)
   POST [Tvoid ]
     PROP ()
     LOCAL ()
-    SEP (mem_mgr gv; nodebox_rep sh (gv _base_root) g_root g) | (!!(sorted_tree (bst_conc_lemmas2.insert x v BST))&& tree_rep2 g g_root (gv _base_root) sh (bst_conc_lemmas2.insert x v BST)).
+    SEP (mem_mgr gv; nodebox_rep sh (gv _base_root) nb g_root g) | (!!(sorted_tree (bst_conc_lemmas2.insert x v BST))&& tree_rep2 g g_op g_root nb sh (bst_conc_lemmas2.insert x v BST)).
 
 Program Definition delete_spec :=
   DECLARE _delete
-  ATOMIC TYPE (rmaps.ConstType ( share* Z * Z * val * globals * gname * gname))
+  ATOMIC TYPE (rmaps.ConstType ( val * share* Z * Z * val * globals * gname * gname * gname))
          OBJ BST INVS base.empty base.top
-  WITH  sh, x,  n, v, gv, g, g_root
+  WITH nb, sh, x,  n, v, gv, g, g_op, g_root
   PRE [ _key OF tint, _thread_num OF tint ]
     PROP (
           Int.min_signed <= x <= Int.max_signed)
     LOCAL (temp _key (Vint (Int.repr x)); temp _thread_num (Vint (Int.repr n)); gvars gv)
-    SEP  (mem_mgr gv; nodebox_rep sh (gv _base_root) g_root g) |(!! sorted_tree BST && tree_rep2 g g_root (gv _base_root) sh BST)
+    SEP  (mem_mgr gv; nodebox_rep sh (gv _base_root) nb g_root g) |(!! sorted_tree BST && tree_rep2 g g_op g_root nb sh BST)
   POST [Tvoid ]
     PROP ()
     LOCAL ()
-    SEP (mem_mgr gv; nodebox_rep sh (gv _base_root) g_root g) | (!!(sorted_tree (bst_conc_lemmas2.delete x BST))&& tree_rep2 g g_root (gv _base_root) sh (bst_conc_lemmas2.delete x BST)).
+    SEP (mem_mgr gv; nodebox_rep sh (gv _base_root) nb g_root g) | (!!(sorted_tree (bst_conc_lemmas2.delete x BST))&& tree_rep2 g  g_op g_root nb sh (bst_conc_lemmas2.delete x BST)).
 
-
- Program Definition helpChildCAS_spec :=
-  DECLARE _helpChildCAS
-  ATOMIC TYPE (rmaps.ConstType ( val * val  * Z * val * Z * val * val * val * val * Z * val * val * share * gname * gname * globals)) OBJ BST INVS base.empty base.top
-  WITH  nb, o, n, d, x, vp, op, lp, rp, b, e, u, sh, g, g_root, gv
-  PRE [  _op OF (tptr t_struct_child_cas_operation), _dest OF  (tptr t_struct_tree),  _thread_num OF tint ]
-          PROP (readable_share sh;Int.min_signed <= x <= Int.max_signed; Int.min_signed <= b <= Int.max_signed)
-          LOCAL (temp _op o; temp _thread_num (Vint (Int.repr n)); temp _dest d; gvars gv )
-          SEP  (mem_mgr gv; data_at sh t_struct_child_cas_operation (Vint (Int.repr b),(e,u)) o; data_at sh t_struct_tree (Vint (Int.repr x),(op,(vp,(lp,rp)))) d; atomic_ptr_at Ews o op (* field_at Ews t_arr (SUB _thread_num) l (gv _rp); listrep Ews lv l *)  ) | (!!(sorted_tree BST)&&tree_rep2 g g_root nb sh BST )
-  POST[ tvoid ]
-  EX o':val,
-        PROP ()
-        LOCAL ()
-       SEP (mem_mgr gv;data_at sh t_struct_child_cas_operation (Vint (Int.repr b),(e,u)) o; data_at sh t_struct_tree (Vint (Int.repr x),(op,(vp,(lp,rp)))) d; atomic_ptr_at Ews o' op (* ;   field_at Ews t_arr (SUB _thread_num) l (gv _rp);  listrep Ews lv' l *) ) | (!!(sorted_tree  BST)&&tree_rep2 g g_root  nb sh BST). 
  
- Program Definition helpMarked_spec :=
+ (* Program Definition helpMarked_spec :=
   DECLARE _helpMarked
   ATOMIC TYPE (rmaps.ConstType ( val * val * Z * val * val * val* val * val * val * Z * val * val * val * val  * Z * share * gname * gname * globals)) OBJ BST INVS base.empty base.top
   WITH  nb, pred, x, vp, op, lp, rp, pred_op, curr, x', vp', op', lp', rp', n, sh, g, g_root, gv
@@ -127,7 +125,7 @@ Program Definition delete_spec :=
         PROP ()
         LOCAL ()
        SEP (mem_mgr gv; data_at sh t_struct_tree (Vint (Int.repr x),(op,(vp,(lp,rp)))) pred; data_at sh t_struct_tree (Vint (Int.repr x'),(op',(vp',(lp',rp')))) curr; atomic_ptr_at Ews o' op (* ;   field_at Ews t_arr (SUB _thread_num) l (gv _rp);  listrep Ews lv' l *) ) | (!!(sorted_tree  BST)&&tree_rep2 g g_root  nb sh BST).
-    Eval  hnf in (reptype t_struct_relocate_operation).
+
 
 Program Definition helpRelocate_spec :=
   DECLARE _helpRelocate
@@ -136,20 +134,20 @@ Program Definition helpRelocate_spec :=
   PRE [  _op OF (tptr t_struct_relocate_operation), _pred OF (tptr t_struct_tree), _pred_op OF  (tptr tvoid), _curr OF (tptr t_struct_tree), _thread_num OF tint ]
           PROP (readable_share sh;Int.min_signed <= x <= Int.max_signed; Int.min_signed <= x' <= Int.max_signed)
           LOCAL (temp _op ro; temp _pred pred;temp _pred_op pred_op; temp _curr curr; temp _thread_num (Vint (Int.repr n));  gvars gv )
-          SEP  (mem_mgr gv;  data_at sh t_struct_relocate_operation (s,(d,(d_op,( Vint(Int.repr rem_k),(Vint(Int.repr rep_key),rep_val ))))) ro; data_at sh t_struct_tree (Vint (Int.repr x),(o,(vp,(lp,rp)))) pred; data_at sh t_struct_tree (Vint (Int.repr x'),(op',(vp',(lp',rp')))) curr (* field_at Ews t_arr (SUB _thread_num) l (gv _rp); listrep Ews lv l *)  ) | (!!(sorted_tree BST)&&tree_rep2 g g_root nb sh BST )
+          SEP  (mem_mgr gv;  @data_at CompSpecs sh t_struct_relocate_operation (s,(d,(d_op,( Vint(Int.repr rem_k),(Vint(Int.repr rep_key),rep_val ))))) ro; @data_at CompSpecs sh t_struct_tree (Vint (Int.repr x),(o,(vp,(lp,rp)))) pred; @data_at CompSpecs sh t_struct_tree (Vint (Int.repr x'),(op',(vp',(lp',rp')))) curr (* field_at Ews t_arr (SUB _thread_num) l (gv _rp); listrep Ews lv l *)  ) | (!!(sorted_tree BST)&&tree_rep2 g g_root nb sh BST )
   POST [tint] 
   EX v:Z,
         PROP ()
-        LOCAL (temp ret_temp v)
-       SEP (mem_mgr gv;  data_at sh t_struct_relocate_operation (s,(d,(d_op,( Vint(Int.repr rem_k),(Vint(Int.repr rep_key),rep_val ))))) ro; data_at sh t_struct_tree (Vint (Int.repr x),(o,(vp,(lp,rp)))) pred; data_at sh t_struct_tree (Vint (Int.repr x'),(op',(vp',(lp',rp')))) curr (* ;   field_at Ews t_arr (SUB _thread_num) l (gv _rp);  listrep Ews lv' l *) ) | ( if eq_dec v 0 then (!!(sorted_tree BST)&&tree_rep2 g g_root nb sh BST ) else (!!(sorted_tree (delete x BST))&&tree_rep2 g g_root  nb sh (delete x BST))). 
-
+        LOCAL (temp ret_temp (vint v))
+       SEP (mem_mgr gv;  data_at sh t_struct_relocate_operation (s,(d,(d_op,( Vint(Int.repr rem_k),(Vint(Int.repr rep_key),rep_val ))))) ro; data_at sh t_struct_tree (Vint (Int.repr x),(o,(vp,(lp,rp)))) pred; data_at sh t_struct_tree (Vint (Int.repr x'),(op',(vp',(lp',rp')))) curr (* ;   field_at Ews t_arr (SUB _thread_num) l (gv _rp);  listrep Ews lv' l *) ) | ( if eq_dec v 0 then (!!(sorted_tree BST)&&tree_rep2 g g_root nb sh BST ) else (!!(sorted_tree (bst_conc_lemmas2.delete rem_k BST))&&tree_rep2 g g_root  nb sh (bst_conc_lemmas2.delete rem_k BST))). 
+ *)
 Definition main_spec :=
  DECLARE _main
   WITH gv : globals
   PRE  [] main_pre prog tt nil gv
   POST [ tint ] main_post prog nil gv.
   
-  Definition acquire_spec := DECLARE _acquire acquire_spec.
+Definition acquire_spec := DECLARE _acquire acquire_spec.
 Definition release2_spec := DECLARE _release2 release2_spec.
 Definition makelock_spec := DECLARE _makelock (makelock_spec _).
 Definition freelock2_spec := DECLARE _freelock2 (freelock2_spec _).
@@ -158,7 +156,7 @@ Definition atomic_load_ptr_spec := DECLARE _atomic_load_ptr (atomic_load_ptr_spe
 Definition atomic_store_ptr_spec := DECLARE _atomic_store_ptr (atomic_store_ptr_spec atomic_ptr atomic_ptr_at).
 Definition atomic_CAS_ptr_spec := DECLARE _atomic_CAS_ptr (atomic_CAS_ptr_spec atomic_ptr atomic_ptr_at).
 Definition make_atomic_ptr_spec := DECLARE _make_atomic_ptr ( make_atomic_ptr_spec atomic_ptr atomic_ptr_at).
-Definition free_atomic_ptr_spec := DECLARE _free_atomic_ptr ( free_atomic_ptr_spec atomic_ptr atomic_ptr_at).
+(* Definition free_atomic_ptr_spec := DECLARE _free_atomic_ptr ( free_atomic_ptr_spec atomic_ptr atomic_ptr_at). *)
 
 Definition Gprog : funspecs :=
     ltac:(with_library prog [acquire_spec; release2_spec; makelock_spec;
@@ -167,14 +165,6 @@ Definition Gprog : funspecs :=
     atomic_store_ptr_spec;
     atomic_CAS_ptr_spec;
     make_atomic_ptr_spec;
-    free_atomic_ptr_spec;
-    (* treebox_new_spec; *)
-    add_spec;
-    find_spec;
-    delete_spec;
-    helpMarked_spec;
-    helpChildCAS_spec;
-    helpRelocate_spec;
     spawn_spec;
     main_spec 
   ]).
@@ -204,21 +194,59 @@ cancel. auto. { unfold sepalg.join. hnf. intro. hnf. simpl. destruct (ghosts.sin
   } auto. auto. 
  Qed.
  
-Definition node_data (info: option ghost_info) g  tp lp rp v (range:number * number)  :=  
-(match info with Some data =>  EX sh, !!(readable_share sh /\ Int.min_signed <= data.1.1.1 <= Int.max_signed/\ is_pointer_or_null lp /\ is_pointer_or_null rp /\ is_pointer_or_null data.1.1.2) && bst.bst_conc_nblocking_spec.atomic_ptr_at Ews v data.1.1.2 * malloc_token Ews t_struct_tree tp * data_at sh t_struct_tree (Vint (Int.repr data.1.1.1),(data.1.1.2,(lp,rp))) tp * in_tree  data.1.2 ( fst range, Finite_Integer (data.1.1.1)) lp g * in_tree data.2 ( Finite_Integer (data.1.1.1), snd range) rp g | None => !!(tp = nullval /\ lp = nullval /\ rp = nullval /\ v = nullval) && emp end).
+Definition node_data (info: option ghost_info) g  tp lp rp aop v (range:number * number)  :=  
+(match info with Some data =>  EX sh, !!(readable_share sh  /\ Int.min_signed <= data.1.1.1 <= Int.max_signed/\ is_pointer_or_null lp /\ is_pointer_or_null rp /\ is_pointer_or_null data.1.1.2 /\  is_pointer_or_null data.1.1.2  ) &&  atomic_ptr_at Ews v data.1.1.2  * malloc_token Ews t_struct_tree tp *
+ data_at sh t_struct_tree (Vint (Int.repr data.1.1.1),(data.1.1.2,(aop,(lp,rp)))) tp * in_tree  data.1.2 ( fst range, Finite_Integer (data.1.1.1)) lp g * in_tree data.2 ( Finite_Integer (data.1.1.1), snd range) rp g | None => !!(tp = nullval /\ lp = nullval /\ rp = nullval /\ v = nullval /\ aop = nullval) && emp end).  
 
-Definition node_information (info: option ghost_info) range g g_current tp lp rp v np  :=  bst.bst_conc_nblocking_spec.atomic_ptr_at Ews tp np * ghost_master1 (ORD := range_order)  (range, info) g_current * 
-node_data info g tp lp rp v range.
+Definition node_information (info: option ghost_info) range g g_current tp lp rp aop v np  :=  atomic_ptr_at Ews tp np * ghost_master1 (ORD := range_order)  (range, info) g_current * 
+node_data info g tp lp rp aop v range.
 
-Lemma node_data_R: forall (info: option ghost_info) g  tp lp rp v (range:number *number),  node_data info g tp  lp rp v range |-- if (eq_dec tp nullval) then !!(info = None /\ lp = nullval /\ rp = nullval /\ v = nullval) && emp  else 
-EX data, EX sh, !!(readable_share sh/\ info = Some data  /\ Int.min_signed <= data.1.1.1 <= Int.max_signed/\ is_pointer_or_null lp /\ is_pointer_or_null rp /\ is_pointer_or_null data.1.1.2) &&  bst.bst_conc_nblocking_spec.atomic_ptr_at Ews v data.1.1.2* malloc_token Ews t_struct_tree tp*  data_at sh t_struct_tree (Vint (Int.repr data.1.1.1),(data.1.1.2,(lp,rp))) tp * in_tree data.1.2( fst range, Finite_Integer data.1.1.1) lp g * in_tree data.2 ( Finite_Integer data.1.1.1, snd range) rp g.
+Lemma node_data_R: forall (info: option ghost_info) g  tp lp rp aop v (range:number *number),  node_data info g tp  lp rp aop v range |-- if (eq_dec tp nullval) then !!(info = None /\ lp = nullval /\ rp = nullval /\ v = nullval) && emp  else 
+EX data, EX sh, !!(readable_share sh/\ info = Some data  /\ Int.min_signed <= data.1.1.1 <= Int.max_signed/\ is_pointer_or_null lp /\ is_pointer_or_null rp /\ is_pointer_or_null data.1.1.2) &&  atomic_ptr_at Ews v data.1.1.2* malloc_token Ews t_struct_tree tp*  data_at sh t_struct_tree (Vint (Int.repr data.1.1.1),(data.1.1.2, ( aop,(lp,rp)))) tp * in_tree data.1.2( fst range, Finite_Integer data.1.1.1) lp g * in_tree data.2 ( Finite_Integer data.1.1.1, snd range) rp g.
 Proof.
-intros. unfold node_data.
+(* intros. unfold node_data.
 destruct info.
 - Intros sh.  assert_PROP (tp <> nullval).  { entailer!. } destruct (eq_dec tp nullval). contradiction. Exists g0 sh. entailer!.
-- Intros. destruct (eq_dec tp nullval). entailer!. contradiction.
-Qed.
+- Intros. destruct (eq_dec tp nullval). entailer!. contradiction. *)
+Admitted.
 
+Definition node_data_op (info: option ghost_info) g g_op  tp lp rp aop op v (range:number * number) (o:option(@operation val)) :=  
+(match info with Some data =>  EX sh, !!(readable_share sh  /\ Int.min_signed <= data.1.1.1 <= Int.max_signed/\ is_pointer_or_null lp /\ is_pointer_or_null rp /\ is_pointer_or_null data.1.1.2 /\  is_pointer_or_null data.1.1.2  ) &&  atomic_ptr_at Ews v data.1.1.2  * malloc_token Ews t_struct_tree tp *
+ atomic_ptr_at Ews op aop * ( match o with |Some o' => in_tree_op g_op o' * match o' with | ADD_op b' x' v' => EX rop, EX t, EX e, EX u,EX vp', EX aop', EX lp', EX rp', EX op', malloc_token Ews t_struct_operation op * data_at Ews t_struct_operation (rop, Vint (Int.repr t)) op * data_at Ews t_struct_child_cas_operation (Vint (Int.repr (if b' then 1 else 0 )), (e, u)) rop
+                                                        * data_at sh t_struct_tree (Vint (Int.repr x'),(vp',(aop',(lp',rp')))) u * atomic_ptr_at Ews v' vp' * atomic_ptr_at Ews op' aop' * data_at Ews t_struct_operation (nullval, Vint (Int.repr 0)) op' * atomic_ptr_at Ews nullval lp' * atomic_ptr_at Ews nullval rp'             
+                                                       | DELETE_op b' x' => EX rop, EX t, malloc_token Ews t_struct_operation op * data_at Ews t_struct_operation (rop, Vint (Int.repr t)) op   end
+                                            |None => emp end) *
+ data_at sh t_struct_tree (Vint (Int.repr data.1.1.1),(data.1.1.2,(aop,(lp,rp)))) tp * in_tree  data.1.2 ( fst range, Finite_Integer (data.1.1.1)) lp g * in_tree data.2 ( Finite_Integer (data.1.1.1), snd range) rp g | None => !!(tp = nullval /\ lp = nullval /\ rp = nullval /\ v = nullval /\ aop = nullval/\ op = nullval ) && emp end).  
+
+Definition node_information_op (info: option ghost_info) range g g_op g_current tp lp rp aop op v np o  :=   atomic_ptr_at Ews tp np * ghost_master1 (ORD := range_order)  (range, info) g_current * 
+node_data_op info g g_op tp lp rp aop op v range o.
+
+Definition node_information_of_child (is_left:bool) (info_parent: option ghost_info) (info_child:option ghost_info) n n0 g  np tp lp rp aop v := match info_parent with 
+| Some data => (atomic_ptr_at Ews tp np *  ghost_master1 (ORD := range_order)  (if is_left then (Finite_Integer data.1.1.1, n0) else (n, Finite_Integer data.1.1.1), info_child) (if is_left then data.1.2 else data.2 ) *
+               (match info_child with |Some data1 => EX sh, !!(readable_share sh /\ Int.min_signed <= data1.1.1.1 <= Int.max_signed/\ is_pointer_or_null lp /\ is_pointer_or_null rp /\ is_pointer_or_null data1.1.1.2 ) && atomic_ptr_at Ews v data1.1.1.2  * malloc_token Ews t_struct_tree tp * atomic_ptr_at Ews nullval aop *  data_at sh t_struct_tree (Vint (Int.repr data1.1.1.1),(data1.1.1.2,(aop,(lp,rp)))) tp * in_tree  data1.1.2 ( (if is_left  then Finite_Integer data.1.1.1 else n), Finite_Integer data1.1.1.1) lp g * in_tree data1.2 ( Finite_Integer data1.1.1.1, (if is_left then n0 else Finite_Integer data.1.1.1)) rp g
+                                     | None => emp end))
+| None =>  emp end. 
+Definition get_range_from_parent (is_left:bool) (n n0:number) (o:option ghost_info) := match o with 
+                  | Some data => if is_left then ( Finite_Integer data.1.1.1, n0) else  (n, Finite_Integer data.1.1.1) 
+                  | None => (n0,n) end.
+Lemma in_tree_delete : forall g s (o:@operation val), in_tree_op g o  * ghost_ref_op g s |-- (|==> ghost_ref_op g (Ensembles.Subtract s o ))%I.
+Proof.
+Admitted.
+
+Lemma extract_node_info_op_from_ghost_tree_rep:  forall  tg np nb g_root g_current g g_op (r_root: number * number) n n0 (o': @operation val) lp rp,
+   Ensembles.In (find_op_set tg ) o' -> (find_ghost_set2 tg g_root r_root nb) g_current = Some (n, n0,np) -> ghost_tree_rep tg nb g_root g g_op r_root  |--  EX tp:val,  EX o:option ghost_info, EX aop: val, EX v:val, EX op,
+    node_information_op o (n, n0) g g_op g_current tp  lp rp aop v np op  ( Some o') * 
+   ( match o' with | ADD_op b' x' v' => node_information_of_child b' o None n n0 g (if b' then rp else lp) nullval nullval nullval nullval nullval *  ((ALL g1 g2:gname,ALL tp1:val, ALL lp1:val, ALL rp1:val, ALL vp:val, ALL aop:val,
+                                        node_information_op o (n, n0) g g_op g_current tp  lp rp aop v np op None * node_information_of_child b' o (Some(x',vp,g1,g2)) n n0 g (if b' then rp else lp) tp1 lp1 rp1 aop v' * node_information_op None (left (get_range_from_parent b' n n0 o), Finite_Integer x') g g_op g1 nullval nullval nullval nullval nullval nullval lp1 None *
+                                       node_information_op None (Finite_Integer x', right(get_range_from_parent b' n n0 o)) g g_op g2 nullval nullval nullval nullval nullval nullval rp1 None) -* (EX tg', !!(find_pure_tree2 tg = find_pure_tree2 tg' /\ find_op_set tg' = Ensembles.Subtract (find_op_set tg) o') && ghost_tree_rep tg' nb g_root g g_op r_root))
+                  | DELETE_op b' x' => EX lp1, EX rp1, EX v, EX aop, EX tp1, EX vp, EX g1, EX g2, node_information_of_child b' o (Some(x',vp,g1,g2)) n n0 g (if b' then rp else lp) tp1 lp1 rp1 aop v * (node_information_op o (n, n0) g g_op g_current tp  lp rp aop v np nullval  None -* (EX tg', !!(find_pure_tree2 tg = find_pure_tree2 tg' /\ find_op_set tg' = Ensembles.Subtract (find_op_set tg) o') && ghost_tree_rep tg' nb g_root g g_op r_root)) end).
+
+Proof.
+intros.
+revert dependent g_root.
+revert dependent r_root.
+induction tg;intros.  
+Admitted.
 
 Lemma ghost_master1_alloc : forall r:node_info,
   emp |-- (|==> (EX g, ghost_master1 r g))%I.
@@ -235,46 +263,46 @@ Qed.
 
 
 Inductive range_info_in_tree (ri: node_info)
-          (range: number * number) (v :val) : ghost_tree -> Prop :=
-| riit_none: (ri = (range, None)) /\ v = nullval -> range_info_in_tree ri range v E_ghost
-| riit_root: forall (l r: ghost_tree) (g1 g2: gname) (lp rp:val) k vp v',
+          (range: number * number) (v :val) : ghost_op_tree -> Prop :=
+| riit_none: (ri = (range, None)) /\ v = nullval -> range_info_in_tree ri range v E_op
+| riit_root: forall (l r: ghost_op_tree) (g1 g2: gname) (lp rp:val) k vp aop o v',
     (ri = (range, Some (k, vp, g1, g2)) /\ v = v')  ->
-    range_info_in_tree ri range v (T_ghost l g1 lp k v' vp r g2 rp)
-| riit_left: forall (l r: ghost_tree) (g1 g2: gname) (lp rp:val) k vp v',
+    range_info_in_tree ri range v (T_op l g1 lp k v' vp aop o r g2 rp)
+| riit_left: forall (l r: ghost_op_tree) (g1 g2: gname) (lp rp:val) k vp aop o v',
     range_info_in_tree ri (range.1, Finite_Integer k) v l ->
-    range_info_in_tree ri range v (T_ghost l g1 lp k v' vp r g2 rp)
-| riit_right: forall (l r: ghost_tree) (g1 g2: gname) (lp rp:val) k vp v',
+    range_info_in_tree ri range v (T_op l g1 lp k v' vp aop o r g2 rp)
+| riit_right: forall (l r: ghost_op_tree) (g1 g2: gname) (lp rp:val) k vp aop o v',
     range_info_in_tree ri (Finite_Integer k, range.2) v r ->
-    range_info_in_tree ri range v (T_ghost l g1 lp k v' vp r g2 rp).
+    range_info_in_tree ri range v (T_op l g1 lp k v' vp aop o r g2 rp).
 
-
-Lemma extract_left_node_info_from_ghost_tree_rep:  forall  tg np b g_root g_current g (r_root: number * number) (range:number*number),
-   (find_ghost_set tg g_root r_root b) g_current = Some (range,np) -> ghost_tree_rep tg b g_root g r_root  |--  EX tp:val,  EX o:option ghost_info, EX lp:val, EX rp:val, EX v:val, 
-   !! range_info_in_tree (range,o) r_root v tg &&  node_information o range g g_current tp  lp rp v np  *
-   ( node_information o range g g_current tp  lp rp v np  -* ghost_tree_rep tg b g_root g r_root).
+(*Lemma extract_node_info_from_ghost_tree_rep:  forall  tg np b g_root g_current g (r_root: number * number) (range:number*number),
+   (find_ghost_set2 tg g_root r_root b) g_current = Some (range,np) -> ghost_tree_rep tg b g_root g r_root  |--  EX tp:val,  EX o:option ghost_info, EX lp:val, EX rp:val, EX aop: val, EX v:val, 
+    node_information o range g g_current tp  lp rp aop v np  *
+   (node_information o range g g_current tp  lp rp aop v np  -* ghost_tree_rep tg b g_root g r_root).
 Proof.
  intros.
 revert dependent b.
 revert dependent g_root.
 revert dependent r_root.
 induction tg;intros. 
-  -  inv H. destruct r_root. destruct range. unfold ghosts.singleton in H1. Exists nullval.  Exists (@None ghost_info) nullval nullval nullval. unfold node_information;simpl. simpl in *. entailer!.
-     { apply  riit_none. destruct (eq_dec g_current g_root). inv H1. split;auto. discriminate. } destruct (eq_dec g_current g_root). inv H1. cancel. rewrite prop_true_andp. apply wand_refl_cancel_right. auto. discriminate.
+  -  inv H. destruct r_root. destruct range. unfold ghosts.singleton in H1. Exists nullval.  Exists (@None ghost_info) nullval nullval nullval nullval. unfold node_information;simpl. simpl in *. entailer!.
+    (*  { apply  riit_none. destruct (eq_dec g_current g_root). inv H1. split;auto. discriminate. } *) destruct (eq_dec g_current g_root). inv H1. cancel. apply wand_frame_intro'. rewrite sepcon_emp;rewrite pull_left_special0. Intros. cancel. discriminate.
   -  intros. simpl in H. unfold map_upd in H. destruct (eq_dec g_current g_root). 
-     * inv H. destruct range. simpl in *.  Intros tp sh . Exists  tp (Some ( k, v1, g0, g1)) v v2 v0. unfold node_information. simpl in *. Exists sh . entailer!.
-       { apply riit_root. split;auto. }  rewrite <- wand_sepcon_adjoint. Intros sh1.  Exists tp sh1. entailer!.
-     * unfold map_add in H. destruct r_root. simpl in *. remember (find_ghost_set tg1 g0 (n0, Finite_Integer k) v g_current) as left_set. destruct left_set.
-        ** Intros rtp sh. sep_apply IHtg1. rewrite <- Heqleft_set. apply H.  Intros tp o lp rp v3 . Exists tp o lp rp v3 . entailer!.
-            { apply  riit_left. auto. }
-             rewrite -> 7sepcon_assoc.  rewrite <- (emp_wand (bst_conc_nblocking_spec.atomic_ptr_at Ews rtp b * _)) . rewrite wand_sepcon_wand. apply wand_derives.
-             rewrite -> sepcon_emp;auto. Exists rtp sh . entailer!.
-        ** Intros rtp sh. sep_apply IHtg2.  Intros tp o lp rp v3 . Exists tp o lp rp v3 . entailer!. 
-            { apply  riit_right. auto. }
-             rewrite -> 7sepcon_assoc.  rewrite <- (emp_wand (bst_conc_nblocking_spec.atomic_ptr_at Ews rtp b * _)) . rewrite wand_sepcon_wand. apply wand_derives.
-             rewrite -> sepcon_emp;auto. Exists rtp sh . entailer!.
+     * inv H. destruct range. simpl in *.  Intros tp op sh . Exists  tp (Some ( k, v1, g0, g1)) v v3 v2 v0. unfold node_information. simpl in *. Exists sh . entailer!.
+       (* { apply riit_root. split;auto. } *) rewrite <- wand_sepcon_adjoint. Intros sh1.  Exists tp op sh1. entailer!.
+     * unfold map_add in H. destruct r_root. simpl in *. remember (find_ghost_set2 tg1 g0 (n0, Finite_Integer k) v g_current) as left_set. destruct left_set.
+        ** Intros rtp op sh. sep_apply IHtg1. rewrite <- Heqleft_set. apply H.  Intros tp o0 lp rp aop v4 . Exists tp o0 lp rp aop v4 . entailer!.
+            (* { apply  riit_left. auto. } *)
+             rewrite -> 8sepcon_assoc.  rewrite <- (emp_wand (atomic_ptr_at Ews rtp b * _)) . rewrite wand_sepcon_wand. apply wand_derives.
+             rewrite -> sepcon_emp;auto. Exists rtp op sh . entailer!.
+        ** Intros rtp op sh. sep_apply IHtg2.  Intros tp o0 lp rp aop v4 . Exists tp o0 lp rp aop v4. entailer!. 
+            (* { apply  riit_right. auto. } *)
+              rewrite -> 8sepcon_assoc.  rewrite <- (emp_wand (atomic_ptr_at Ews rtp b * _)) . rewrite wand_sepcon_wand. apply wand_derives.
+             rewrite -> sepcon_emp;auto. Exists rtp op sh . entailer!.
+Qed. 
 
-Qed.
-
+*)
+(*
 Lemma range_info_in_tree_In: forall tg x vp ga gb range v r_root,
     range_info_in_tree (range,  Some (x, vp, ga, gb)) r_root v tg ->
    bst.bst_conc_lemmas.In x (find_pure_tree tg).
@@ -469,8 +497,7 @@ induction tg.
             +++ apply allp_right; intro g2. apply allp_right;intro g3. apply allp_right;intro v5. repeat (rewrite allp_sepcon2; eapply allp_left). instantiate(1:= g2).  instantiate(1:= g3).  instantiate(1:= v5). 
                   rewrite <- wand_sepcon_adjoint. assert_PROP (check_key_exist' x (n, n0) = true). { simpl. entailer!. } 
                  simpl in H3.  apply andb_prop in H4. apply andb_prop in H1.  destruct H4, H1. destruct n. simpl in H1. apply Z.ltb_lt in H1. apply Zle_bool_imp_le in H4. omega. discriminate. simpl in H1. discriminate.     
-Qed.
+Qed. *)
 
-  End Specifications.
 
   
